\documentclass[aps,12pt]{revtex4}
\usepackage[a4paper]{geometry}
\usepackage{graphicx}
\usepackage{amssymb,amsfonts,amsmath,amsthm}
\usepackage{bm}
\usepackage{pslatex}
\usepackage{chemarr}
\usepackage{mathptmx}
\usepackage{bookman}


\begin{document}

Let us assume that we have three points $a\leq b \leq c$ and their values
$f_a,f_b,f_c$ such that
\begin{equation}
	f_b \leq f_a \text{ and } f_b \leq f_c
\end{equation} 

We rescale the problem with
$$
	a \to 0, b \to \beta, c \to 1
$$	

$$
	g_0 = f_a - f_b \geq 0, \;\; g_1 = f_c - f_b \geq 0
$$

$$
	g(u) = (1-u) f_0 + u f_1 - \lambda u(1-u)
$$
$$
	0 = (1-\beta) g_0 + \beta g_1 - \lambda \beta(1-\beta)
$$

$$
	\lambda = \dfrac{(1-\beta) g_0 + \beta g_1 }{\beta(1-\beta)}
$$

$$
	g'(u) = g_1-g_0 + \lambda (2u-1)
$$

$$
	u_m = \dfrac{1}{2} \dfrac{\lambda - (g_1-g_0)}{\lambda} = \dfrac{1}{2}\left[ 1 + \dfrac{g_0-g_1}{\lambda} \right]
$$

$$
	u_m = \frac{1}{2} \left[ 1 + \dfrac{ \beta(1-\beta) (g_0-g_1) }{ (1-\beta) g_0 + \beta g_1 } \right]
$$



\end{document}